ECCA/typing_lemmas.v
@@ -1,23 +1,127 @@
 Require Export typing.
 
-(* Open Scope ECCA_scope.
+Open Scope ECCA_scope.
 Theorem weakening {Γ e A}:
-  (Γ |- e : A) ->
+  (Γ ⊢ e : A) ->
   forall r Δ,
     Γ =[r]=> Δ ->
-    (Δ |- ([r] e) : A).
+    (Δ ⊢ ([r] e) : A).
 Proof.
-Admitted. *)
+Admitted.
+
+Lemma weakening1 (g: env) (A U B: exp) (x: name):
+(g ⊢ A : U) ->
+(g & x ~ Assum B ⊢ [^x] A : U) /\ (forall e: exp, (g & x ~ Def e B ⊢ [^x] A : U)).
+Proof.
+Admitted.
+
+
+
+Require Import String.
+Open Scope string.
+
+Lemma WF_1: 
+(⊢ (ctx_empty & "x" ~ Def eBool (eUni (uType 0)))).
+Proof. eapply wf_Def; auto.
+Qed.
+
+Lemma WF_2:
+(⊢(ctx_empty & "x" ~ Def eBool (eUni (uType 0)) & "y" ~ Assum (eId (free "x")))).
+Proof. eapply wf_Assum. apply WF_1. apply aT_Var; eauto with contexts.
+Qed.
+
+Lemma WF_3:
+(⊢((((ctx_empty & "x" ~ Def eBool (eUni (uType 0))
+            & "y" ~ Assum (eId (free "x")))
+            & "x" ~ Def (eUni uProp) (eUni (uType 0)))))).
+Proof. eapply wf_Def. apply WF_2.
+  - apply aT_Ax_Type. apply WF_2.
+  - apply aT_Ax_Prop. apply WF_2.
+Qed.
+
+Lemma typing_is_broken_part_1: 
+((ctx_empty & "x" ~ Def eBool (eUni (uType 0)) & "y" ~ Assum (eId (free "x"))) ⊢ eId (free "y") : eBool).
+Proof.
+eapply aT_Conv.
++ apply aT_Var.
+  - apply WF_2. 
+  - left. auto with contexts.
++ apply aT_Bool. eapply wf_Assum.
+  - eapply wf_Def.
+    * auto.
+    * auto.
+    * auto.
+  - apply aT_Var; eauto with contexts.
++ apply ST_Cong. apply aE_Step with (e:=eBool).
+  - apply R_RedR. apply st_ID with (A:= (eUni (uType 0))); auto with contexts.
+  - apply R_Reflex.
+Qed.
+
+Lemma typing_is_broken_part_2: 
+(((ctx_empty & "x" ~ Def eBool (eUni (uType 0))
+            & "y" ~ Assum (eId (free "x")))
+            & "x" ~ Def (eUni uProp) (eUni (uType 0))) ⊢ eId (free "y") : (eUni uProp)).
+Proof.
+eapply aT_Conv.
++ apply aT_Var. apply WF_3. left. auto with contexts.
++ apply aT_Ax_Prop. apply WF_3.
++ apply ST_Cong. apply aE_Step with (e:=eUni uProp).
+  - apply R_RedR. apply st_ID with (A:= (eUni (uType 0))). auto with contexts.
+  - apply R_Reflex.
+Qed.
+
+
+(* Conclusion: We need to shift the bodies of ass/defs in the context when we add a new ass/def *)
+
+Lemma WellFormed_implies (g: env) (A: exp):
+WellFormed g ->
+forall (x: name),
+assumes g (free x) A ->
+exists U, Types g ([^x]A) U.
+Proof.
+induction g. 
+ - intros. inversion H0. inversion H1. inversion H1. inversion H2.
+ - intros. inversion H. subst. inversion H0.
+   cbn in H1. destruct (closev a (free x)). Admitted.
+   
+
+
+(* H1.
+  + cbn in H1. destruct (bindv (closev x (free x0))).
+    * cut (assumes g v A).
+      -- intros. cut (exists n, v = free n).
+         ** intros. destruct H3. subst. apply IHWellFormed in H2. destruct H2. exists x2. apply weakening1. auto. 
+      -- auto.
+    * inversion H1. subst. exists U. apply weakening1. auto.
+  + cbn in H1. destruct (bindv (closev x x0)).
+    * cut (assumes g v A).
+      -- intros. apply IHWellFormed in H2. destruct H2. exists x1. apply weakening1. auto. 
+      -- auto.
+    * inversion H1. inversion H2.
+  - intros. destruct H2.
+    + cbn in H2. destruct (bindv (closev x x0)).
+      * cut (assumes g v A).
+        -- intros. apply IHWellFormed in H3. destruct H3. exists x1. apply weakening1. auto. 
+        -- auto.
+      * inversion H2.
+    + cbn in H2. destruct (bindv (closev x x0)).
+      * cut (assumes g v A).
+        -- intros. apply IHWellFormed in H3. destruct H3. exists x1. apply weakening1. auto. 
+        -- auto.
+      * inversion H2. inversion H3. subst. exists U. apply weakening1. auto.
+Qed. *)
+
+
 
 Lemma type_well_typed (g: env) (N: exp) (A: exp) :
-  Types g N A ->
-  WellFormed g ->
+  (g ⊢ N : A) ->
+  (⊢ g) ->
   exists U , Types g A U.
 Proof.
   induction 1.
   - exists (eUni (uType 1)). apply aT_Ax_Type. auto.
   - exists (eUni (uType (S (S i)))). apply aT_Ax_Type. auto.
-  - intros. induction H0.
+  - intros. Admitted. (*  apply WellFormed_implies. intros. induction H0.
     + subst. destruct H; destruct h. 
     + subst. destruct H. cbn in h. destruct (bindv (closev x0 x)).
       * names.  
@@ -35,13 +139,13 @@ Proof.
   - shelve.
   - shelve.
   - shelve. 
-Admitted. 
+Admitted.  *)
 
 Lemma has_type_wf_g (g: env) (N: exp) (A: exp) (x : name):
   Types g N A ->
   WellFormed g ->
   WellFormed (g & x ~ (Def N A)).
 Proof.
-  intros.  apply type_well_typed in H as H1. destruct H1.
+  intros.  apply type_well_typed in H as H1; auto. destruct H1.
   apply wf_Def with (U := x0); auto.
 Qed. 
