translation/trans_preservation.v
@@ -1,31 +1,37 @@
 Require Import ECC.
 Require Import ECCA.core ECCA.typing ECCA.equiv ECCA.continuations.
 Require Import translator.
-Require Import ECCA.key_lemmas.
-(* 
-Definition P1 (g : ECC.env) (e A : ECC.exp) (h : ECC.Types g e A) :=
-  forall (g': ECCA.core.env) (K: cont_r) (B N: ECCA.core.exp),
-    ECCA_cont_has_type (appendEnv (transEnv g) g') (unrestrict_cont K) (Cont N (flattenECCAconf (trans A)) B) ->
-    ECCA_Equiv (appendEnv (transEnv g) g') (flattenECCAconf (trans e)) N ->
-    ECCA.typing.Types (appendEnv (transEnv g) g') (unrestrict_conf (transWork (ECC.FV e) e K)) B.
+From Equations Require Import Equations.
+(* Require Import ECCA.key_lemmas. *)
 
-Definition P2 (g : ECCenv) (h : ECC_Env_WF g) := ECCA_Env_WF (transEnv g).
+
+Definition P1 (g : ECC.env) (e A : ECC.exp) (h : ECC.Types g e A) :=
+forall (g' : env) (K : cont),
+cont_is_ANF K ->
+forall B N : exp,
+(append (translateEnv g) g' ⊩ K : (〔 N : [[A]] 〕 ⇒ B))%ECCA ->
+(append (translateEnv g) g' ⊢ [[e]] ≡ N)%ECCA ->
+(append (translateEnv g) g' ⊢ translate e K : B)%ECCA.
+
+Definition P2 (g : ECC.env) (h : ECC.WellFormed g) := (⊢ translateEnv g)%ECCA.
 
 Lemma strong_trans_preservation :
-  (forall (g : ECCenv) (h : ECC_Env_WF g),  ECCA_Env_WF (transEnv g))
-  /\
-  (forall (g : ECCenv) (e A : ECCexp) (H : ECC_has_type g e A),
-      forall (g': ECCAenv) (K: cont_r)
-             (B N: ECCAexp),
-        ECCA_cont_has_type (appendEnv (transEnv g) g') (unrestrict_cont K) (Cont N (flattenECCAconf (trans A)) B) ->
-        ECCA_Equiv (appendEnv (transEnv g) g') (flattenECCAconf (trans e)) N ->
-        ECCA_has_type (appendEnv (transEnv g) g') (flattenECCAconf (transWork (ECC.FV e) e K)) B).
-Proof.
+(forall g : ECC.env, (⊢ g)%ECC -> (⊢ translateEnv g)%ECCA) 
+/\
+(forall (g : ECC.env) (e A : ECC.exp),
+  (g ⊢ e : A)%ECC ->
+  forall (g' : env) (K : cont),
+    cont_is_ANF K ->
+    forall B N : exp,
+      (append (translateEnv g) g' ⊩ K : (〔 N : [[A]] 〕 ⇒ B))%ECCA ->
+      (append (translateEnv g) g' ⊢ [[e]] ≡ N)%ECCA ->
+      (append (translateEnv g) g' ⊢ translate e K : B)%ECCA).
+Proof. 
 intros.
-simple apply ECC_type_env_comb; intros.
-- unfold transWork. simpl.  destruct (atom_fresh empty). destruct (atom_fresh (add x empty)). destruct (atom_fresh (add x0 (add x empty))).
+simple apply ECC.type_env_comb; intros.
++ simp translate. 
+(* - simp translate. destruct (atom_fresh empty). destruct (atom_fresh (add x empty)). destruct (atom_fresh (add x0 (add x empty))).
   cut (ECCA_has_type (transEnv g) (Uni uProp) (Uni (uType 0))).
   + shelve. (*eapply Cut. *)
-  + auto.
+  + auto. *)
 Admitted.
- *)
